Primitive rules ... reproved with new tactics

theories/vir/rules/primitive_laws.v
@@ -7,9 +7,6 @@ From velliris.vir.lang Require Export lang.
 
 From ITree.Events Require Import State StateFacts.
 
-(* From ITree Require Import *)
-(*   ITree Eq.Eqit Eq.EqAxiom Events.State Events.StateFacts Extra.IForest. *)
-(* From Vellvm Require Import Semantics.LLVMEvents Handlers.Handlers Handlers.MemoryTheory. *)
 Set Default Proof Using "Type*".
 
 Ltac itree_state_simp e :=
@@ -54,7 +51,28 @@ Ltac tgt_final :=
         iApply target_red_base
    end.
 
-Section proof.
+(* ------------------------------------------------------------------------ *)
+(* Utility  *)
+(* ------------------------------------------------------------------------ *)
+
+Lemma read_logical_view m ptr n b o τ:
+  (⊙ m) !! ptr.1 = Some (LBlock n b o) ->
+  read m ptr τ = inr (read_in_mem_block b (snd ptr) τ).
+Proof.
+  intros Hs.
+  apply get_logical_block_logical_view in Hs.
+  rewrite /read. setoid_rewrite Hs. reflexivity.
+Qed.
+
+Definition update_block (b : logical_block) (f : mem_block -> mem_block) : logical_block :=
+  match b with
+    | LBlock n m i => LBlock n (f m) i
+  end.
+
+(* ======================================================================== *)
+(* Primitive laws on instruction-related events. *)
+
+Section primitive_rules.
 
   Context {Σ} `{!vellirisGS Σ}.
 
@@ -63,7 +81,11 @@ Section proof.
 
   Local Ltac final := src_final; tgt_final; done.
 
-  Lemma source_red_alloca τ `{non_void τ} Ψ S_s i:
+  (* ------------------------------------------------------------------------ *)
+  (* Source-side primitive laws on instruction-related events *)
+  (* ------------------------------------------------------------------------ *)
+
+  Lemma source_alloca τ `{non_void τ} Ψ S_s i:
     alloca_src i S_s -∗
     stack_src i -∗
     (∀ z,
@@ -111,7 +133,267 @@ Section proof.
     destruct f; cbn -[frame_at]; iFrame.
   Qed.
 
-  Lemma target_red_alloca τ `{non_void τ} Ψ S_s i:
+  Lemma source_load_block ptr τ Ψ q n b o:
+    ptr.1 ↦{q}s [ LBlock n b o ] -∗
+    (ptr.1 ↦{q}s [ LBlock n b o ] -∗
+      Ψ (Ret (read_in_mem_block b (snd ptr) τ))) -∗
+    source_red (η := vir_handler) (trigger (Load τ (DVALUE_Addr ptr))) Ψ.
+  Proof.
+    rewrite source_red_unfold.
+    iIntros "Hs Hl". iLeft.
+    iIntros (σ_t σ_s) "SI".
+    iDestruct "SI" as (???) "(Hh_s & Hh_t & H_c & Hbij & SI)".
+
+    iPoseProof (heap_read_st_1 with "Hh_s Hs") as "%lookup".
+    cbn in *; eapply (read_logical_view _ _ _ _ _ τ) in lookup.
+
+    iModIntro.
+    iExists _,
+      (read_in_mem_block b (snd ptr) τ),
+      (fun x => Tau (Ret x)),σ_s. iFrame. (* Long processing time *)
+    iSpecialize ("Hl" with "Hs").
+    iSplitL ""; first iPureIntro.
+    { solve_eq. rewrite lookup //=. tau_steps.
+      solve_eq. rewrite update_mem_id.
+      reflexivity. }
+    iSplitR "Hl"; last final; sfinal.
+  Qed.
+
+  Corollary source_load_block1 ptr τ Ψ q b:
+    ptr.1 ↦{q}s [ b ] -∗
+    (ptr.1 ↦{q}s [ b ] -∗
+      Ψ (Ret (read_in_mem_block (lb_mem b) (snd ptr) τ))) -∗
+    source_red (η := vir_handler) (trigger (Load τ (DVALUE_Addr ptr))) Ψ.
+  Proof.
+    destruct b.
+    iApply source_load_block.
+  Qed.
+
+  Lemma source_load l τ v Ψ q :
+    is_supported τ ->
+    dvalue_has_dtyp v τ  ->
+    l ↦{q}s v -∗
+    (l ↦{q}s v -∗ Ψ (Ret (dvalue_to_uvalue v))) -∗
+    source_red (η := vir_handler) (trigger (Load τ (# l))) Ψ.
+  Proof.
+    rewrite source_red_unfold.
+    iIntros (Hs Hτ) "Hs Hl". iLeft.
+    iIntros (σ_t σ_s) "SI".
+    iDestruct "SI" as (???) "(Hh_s & Hh_t & H_c & Hbij & %WF & SI)".
+
+    iPoseProof (heap_read with "Hh_s Hs") as "%lookup".
+    cbn.
+    pose proof (read_uvalue_logical_view _ _ _ _ Hs Hτ lookup) as Hread.
+
+    iModIntro.
+    iExists _,
+      (dvalue_to_uvalue v),
+      (fun x => Tau (Ret x)), σ_s. iFrame. (* Long processing time *)
+    iSpecialize ("Hl" with "Hs").
+    iSplitL ""; first iPureIntro.
+    { solve_eq. cbn; rewrite Hread.
+      solve_eq. by rewrite update_mem_id. }
+    iSplitR "Hl"; last final; sfinal.
+  Qed.
+
+  Lemma source_store_block v v' n i Ψ ptr:
+    ptr.1 ↦s [ LBlock n v i ] -∗
+    (ptr.1 ↦s [ LBlock n (add_all_index (serialize_dvalue v') ptr.2 v) i ] -∗
+      Ψ (Ret tt)) -∗
+    source_red (η := vir_handler) (trigger (Store (DVALUE_Addr ptr) v')) Ψ.
+  Proof.
+    rewrite source_red_unfold.
+    iIntros "Hs Hl". iLeft.
+    iIntros (σ_t σ_s) "SI".
+    iDestruct "SI" as (???) "(Hh_s & Hh_t & H_c & Hbij & SI)".
+
+    iDestruct (heap_read_st_1 with "Hh_s Hs") as %?; auto.
+    iPoseProof (heap_write with "Hh_s Hs") as ">(Hh_s & Hs)".
+    cbn. destruct ptr.
+    iSpecialize ("Hl" with "Hs").
+
+    iModIntro.
+    iExists _,tt,(fun x => Tau(Ret x)),_.
+    iSplitL ""; first iPureIntro.
+    { solve_eq.
+      apply get_logical_block_logical_view in H. rewrite /write.
+      rewrite /vir_heap in H. rewrite /get_logical_block /get_logical_block_mem.
+      rewrite H; cbn. by solve_eq. }
+
+    iSplitR "Hl"; last final; sfinal.
+
+    cbn; rewrite <- vir_heap_add_logical_block. cbn.
+    rewrite /dvalue_to_block.
+    cbn in *. rewrite /frames; cbn; eauto.
+    destruct_HC "Hh_s".
+
+    assert ({[ z ]} ∪ (vmem σ_s).1.2 = (vmem σ_s).1.2).
+    { destruct Hbs. cbn in *.
+      specialize (H1 z (ltac:(rewrite lookup_insert; eauto))).
+      destruct H1. set_solver. }
+
+    destruct (vmem σ_s); destruct f; cbn in *;
+    rewrite H0; sfinal.
+  Qed.
+
+  Lemma source_store v v' l Ψ:
+    length (serialize_dvalue v) = length (serialize_dvalue v') ->
+    l ↦s v -∗
+    (l ↦s v' -∗ Ψ (Ret tt)) -∗
+    source_red (η := vir_handler) (trigger (Store (# l) v')) Ψ.
+  Proof.
+    rewrite source_red_unfold.
+    iIntros (Hlen) "Hs Hl". iLeft.
+    iIntros (σ_t σ_s) "SI".
+    iDestruct "SI" as (???) "(Hh_s & Hh_t & H_c & Hbij & SI)".
+
+    iDestruct (heap_read with "Hh_s Hs") as %?; auto.
+    rewrite mapsto_dval_eq /mapsto_dval_def.
+    iPoseProof (heap_write with "Hh_s Hs") as ">(Hh_s & Hs)".
+    cbn; iSpecialize ("Hl" with "Hs").
+
+    iModIntro. iExists _,tt,(fun x => Tau (Ret x)),_.
+    iSplitL ""; first iPureIntro.
+    { solve_eq.
+      rewrite /write; rewrite get_logical_block_logical_view in H.
+      rewrite H. by solve_eq. }
+
+    iSplitR "Hl"; last final; sfinal.
+
+    cbn; rewrite <- vir_heap_add_logical_block.
+    rewrite /dvalue_to_block.
+    apply Nat2Z.inj_iff in Hlen. do 2 rewrite <- Zlength_correct in Hlen.
+
+    epose proof (@add_all_index_twice _ _ _ _ _ 0
+        (init_block (N.of_nat (length (serialize_dvalue v)))) Hlen).
+    apply leibniz_equiv in H0. rewrite H0.
+    rewrite !Zlength_correct in Hlen.
+    apply Nat2Z.inj in Hlen. rewrite Hlen.
+    rewrite /frames.
+    destruct (vmem σ_s) ; cbn in *.
+
+    destruct_HC "Hh_s".
+
+    assert ({[ l ]} ∪ p.2 = p.2).
+    { destruct Hbs. cbn in *.
+      destruct p. cbn in *.
+      specialize (H2 l (ltac:(rewrite lookup_insert; eauto))).
+      set_solver. }
+    rewrite H1.
+    sfinal.
+  Qed.
+
+  Corollary source_store_block1 b v' Ψ ptr:
+    ptr.1 ↦s [ b ] -∗
+    (ptr.1 ↦s [ update_block b
+                  (fun v => add_all_index (serialize_dvalue v') ptr.2 v) ] -∗
+      Ψ (Ret tt)) -∗
+    source_red (η := vir_handler) (trigger (Store (DVALUE_Addr ptr) v')) Ψ.
+  Proof.
+    destruct b; iApply source_store_block.
+  Qed.
+
+  Lemma source_local_read (x : LLVMAst.raw_id) (v : uvalue) i Ψ:
+    ⊢ [x := v]s i -∗
+      stack_src i -∗
+      ([x := v]s i -∗
+        stack_src i -∗
+        Ψ (Ret v)) -∗
+      source_red (η := vir_handler) (trigger (LocalRead x)) Ψ.
+  Proof.
+    rewrite source_red_unfold.
+    iIntros "Hl Hf H".
+    iLeft.
+    iIntros (σ_t σ_s) "SI".
+
+    iDestruct "SI" as (???) "(Hh_s & Hh_t & H_c & Hbij & SI)".
+
+    iDestruct (lheap_lookup with "Hh_s Hf Hl") as %Ht.
+    rewrite -alist_find_to_map_Some in Ht.
+
+    iExists _, v, (fun x => Tau(Ret x)), _.
+
+    destruct (vlocal σ_s) eqn: Hσ_s.
+    iSplitL ""; first iPureIntro.
+    { solve_eq.
+      rewrite Hσ_s. cbn. rewrite Ht.
+      solve_eq.
+      by rewrite -Hσ_s update_local_id. }
+
+    iSpecialize ("H" with "Hl Hf").
+    iSplitR "H"; last final.
+
+    repeat iExists _; rewrite Hσ_s; by iFrame.
+  Qed.
+
+  Lemma source_local_write_alloc
+    (x : LLVMAst.raw_id) (v : uvalue) L i Φ :
+    x ∉ L ->
+    ⊢ ldomain_src i L -∗
+      stack_src i -∗
+      ([ x := v ]s i -∗
+        ldomain_src i ({[x]} ∪ L) -∗
+          stack_src i -∗
+          Φ (Ret tt)) -∗
+      source_red (η := vir_handler) (trigger (LocalWrite x v)) Φ.
+  Proof.
+    rewrite source_red_unfold.
+    iIntros (Hlen) "Hd Hf Hl"; iLeft; iIntros (σ_t σ_s) "SI".
+
+    iDestruct "SI" as (???) "(Hh_s & Hh_t & H_c & Hbij & SI)".
+    destruct (vlocal σ_s) eqn: Hlocal_s.
+
+    iExists _,
+      (update_local (alist_add x v l, l0) σ_s),
+      (fun x => Tau (Ret tt)),_.
+
+    iSplitL ""; first iPureIntro.
+    { solve_eq; rewrite Hlocal_s; by solve_eq. }
+
+    iMod ((lheap_domain_alloc _ _ v)
+           with "Hd Hf Hh_s") as "(Hh_s & Hp_s & Hf_s & Hd_s)"; [done | ].
+
+    iDestruct (lheap_lookup with "Hh_s Hf_s Hp_s") as %Hl_s; cbn; iFrame.
+
+    iSpecialize ("Hl" with "Hp_s Hd_s Hf_s"); iFrame.
+    iSplitR "Hl"; last final; sfinal.
+  Qed.
+
+  Lemma source_local_write
+    (x : LLVMAst.raw_id) (v v' : uvalue) i Φ :
+    ⊢ [ x := v' ]s i -∗
+      stack_src i -∗
+      ([ x := v ]s i -∗
+          stack_src i -∗
+          Φ (Ret tt)) -∗
+      source_red (η := vir_handler) (trigger (LocalWrite x v)) Φ.
+  Proof.
+    rewrite source_red_unfold.
+    iIntros "Hx Hf Hl"; iLeft; iIntros (σ_t σ_s) "SI".
+
+    iDestruct "SI" as (???) "(Hh_s & Hh_t & H_c & Hbij & SI)".
+    destruct (vlocal σ_s) eqn: Hlocal_s.
+
+    iExists _,
+      (update_local (alist_add x v l, l0) σ_s),
+      (fun x => Tau (Ret tt)),_.
+
+    iSplitL ""; first iPureIntro.
+    { solve_eq. rewrite Hlocal_s. by solve_eq. }
+
+    iMod ((lheap_write _ _ _ v) with "Hh_s Hf Hx") as "(Hh_s & Hf & Hx)".
+
+    iDestruct (lheap_lookup with "Hh_s Hf Hx") as %Hl_s; cbn.
+
+    iSpecialize ("Hl" with "Hx Hf"); iFrame.
+    iSplitR "Hl"; last final; sfinal.
+  Qed.
+
+  (* ------------------------------------------------------------------------ *)
+  (* Target-side primitive laws on instruction-related events *)
+  (* ------------------------------------------------------------------------ *)
+
+  Lemma target_alloca τ `{non_void τ} Ψ S_s i:
     alloca_tgt i S_s -∗
     stack_tgt i -∗
     (∀ z,
@@ -164,73 +446,7 @@ Section proof.
     destruct f; cbn -[frame_at]; iFrame.
   Qed.
 
-  Lemma sim_alloca τ S_t S_s i_t i_s `{non_void τ}:
-    alloca_tgt i_t S_t -∗
-    alloca_src i_s S_s -∗
-    stack_tgt i_t -∗
-    stack_src i_s -∗
-    trigger (Alloca τ) ⪯ trigger (Alloca τ)
-      [{ (a, a0),
-          ∃ l_t l_s,
-            ⌜a = DVALUE_Addr (l_t, 0%Z)⌝ ∗ ⌜a0 = DVALUE_Addr (l_s, 0%Z)⌝ ∗
-            ⌜l_t ∉ S_t⌝ ∗ ⌜l_s ∉ S_s⌝ ∗
-            l_t ↦t [ make_empty_logical_block τ ] ∗
-            l_s ↦s [ make_empty_logical_block τ ] ∗
-            alloca_tgt i_t ({[l_t]} ∪ S_t) ∗
-            alloca_src i_s ({[l_s]} ∪ S_s) ∗
-            stack_tgt i_t ∗
-            stack_src i_s ∗
-            target_block_size l_t (Some (N.to_nat (sizeof_dtyp τ))) ∗
-            source_block_size l_s (Some (N.to_nat (sizeof_dtyp τ)))}].
-  Proof.
-    iIntros "Hl_t Hl_s Hf_t Hf_s".
-    iApply target_red_sim_expr.
-    iApply (target_red_alloca with "Hl_t Hf_t"); [ done | ].
-    iIntros (??) "Hl_t Ha_t Hf_t Hb_t".
-
-    iApply source_red_sim_expr.
-    iApply (source_red_alloca with "Hl_s Hf_s"); [ done | ].
-    iIntros (??) "Hl_s Ha_s Hf_s Hb_s".
-
-    vfinal. sfinal.
-  Qed.
-
-  Lemma read_logical_view m ptr n b o τ:
-    (⊙ m) !! ptr.1 = Some (LBlock n b o) ->
-    read m ptr τ = inr (read_in_mem_block b (snd ptr) τ).
-  Proof.
-    intros Hs.
-    apply get_logical_block_logical_view in Hs.
-    rewrite /read. setoid_rewrite Hs. reflexivity.
-  Qed.
-
-  Lemma source_red_load1 ptr τ Ψ q n b o:
-    ptr.1 ↦{q}s [ LBlock n b o ] -∗
-    (ptr.1 ↦{q}s [ LBlock n b o ] -∗
-      Ψ (Ret (read_in_mem_block b (snd ptr) τ))) -∗
-    source_red (η := vir_handler) (trigger (Load τ (DVALUE_Addr ptr))) Ψ.
-  Proof.
-    rewrite source_red_unfold.
-    iIntros "Hs Hl". iLeft.
-    iIntros (σ_t σ_s) "SI".
-    iDestruct "SI" as (???) "(Hh_s & Hh_t & H_c & Hbij & SI)".
-
-    iPoseProof (heap_read_st_1 with "Hh_s Hs") as "%lookup".
-    cbn in *; eapply (read_logical_view _ _ _ _ _ τ) in lookup.
-
-    iModIntro.
-    iExists _,
-      (read_in_mem_block b (snd ptr) τ),
-      (fun x => Tau (Ret x)),σ_s. iFrame. (* Long processing time *)
-    iSpecialize ("Hl" with "Hs").
-    iSplitL ""; first iPureIntro.
-    { solve_eq. rewrite lookup //=. tau_steps.
-      solve_eq. rewrite update_mem_id.
-      reflexivity. }
-    iSplitR "Hl"; last final; sfinal.
-  Qed.
-
-  Lemma target_red_load1 ptr τ Ψ q n b o:
+  Lemma target_load_block ptr τ Ψ q n b o:
     ptr.1 ↦{q}t [ LBlock n b o ] -∗
     (ptr.1 ↦{q}t [ LBlock n b o ] -∗
       Ψ (Ret (read_in_mem_block b (snd ptr) τ))) -∗
@@ -256,54 +472,16 @@ Section proof.
     iSplitR "Hl"; last final; sfinal.
   Qed.
 
-  Corollary source_red_load2 ptr τ Ψ q b:
-    ptr.1 ↦{q}s [ b ] -∗
-    (ptr.1 ↦{q}s [ b ] -∗
-      Ψ (Ret (read_in_mem_block (lb_mem b) (snd ptr) τ))) -∗
-    source_red (η := vir_handler) (trigger (Load τ (DVALUE_Addr ptr))) Ψ.
-  Proof.
-    destruct b.
-    iApply source_red_load1.
-  Qed.
-
-  Corollary target_red_load2 ptr τ Ψ q b:
+  Corollary target_load_block1 ptr τ Ψ q b:
     ptr.1 ↦{q}t [ b ] -∗
     (ptr.1 ↦{q}t [ b ] -∗
       Ψ (Ret (read_in_mem_block (lb_mem b) (snd ptr) τ))) -∗
     target_red (η := vir_handler) (trigger (Load τ (DVALUE_Addr ptr))) Ψ.
   Proof.
-    destruct b.
-    iApply target_red_load1.
+    destruct b; iApply target_load_block.
   Qed.
 
-  Lemma source_red_load l τ v Ψ q :
-    is_supported τ ->
-    dvalue_has_dtyp v τ  ->
-    l ↦{q}s v -∗
-    (l ↦{q}s v -∗ Ψ (Ret (dvalue_to_uvalue v))) -∗
-    source_red (η := vir_handler) (trigger (Load τ (# l))) Ψ.
-  Proof.
-    rewrite source_red_unfold.
-    iIntros (Hs Hτ) "Hs Hl". iLeft.
-    iIntros (σ_t σ_s) "SI".
-    iDestruct "SI" as (???) "(Hh_s & Hh_t & H_c & Hbij & %WF & SI)".
-
-    iPoseProof (heap_read with "Hh_s Hs") as "%lookup".
-    cbn.
-    pose proof (read_uvalue_logical_view _ _ _ _ Hs Hτ lookup) as Hread.
-
-    iModIntro.
-    iExists _,
-      (dvalue_to_uvalue v),
-      (fun x => Tau (Ret x)), σ_s. iFrame. (* Long processing time *)
-    iSpecialize ("Hl" with "Hs").
-    iSplitL ""; first iPureIntro.
-    { solve_eq. cbn; rewrite Hread.
-      solve_eq. by rewrite update_mem_id. }
-    iSplitR "Hl"; last final; sfinal.
-  Qed.
-
-  Lemma target_red_load l τ v Ψ q :
+  Lemma target_load l τ v Ψ q :
     is_supported τ ->
     dvalue_has_dtyp v τ  ->
     l ↦{q}t v -∗
@@ -330,119 +508,7 @@ Section proof.
     iSplitR "Hl"; last final; sfinal.
   Qed.
 
-  Lemma sim_load l_t l_s τ v_t v_s q_t q_s:
-    is_supported τ ->
-    dvalue_has_dtyp v_t τ  ->
-    dvalue_has_dtyp v_s τ  ->
-    l_t ↦{q_t}t v_t -∗ l_s ↦{q_s}s v_s -∗
-    trigger (Load τ (# l_t)) ⪯ trigger (Load τ (# l_s))
-      [{ (uv_t, uv_s),
-            ⌜uvalue_to_dvalue uv_t = inr v_t⌝ ∗
-            ⌜uvalue_to_dvalue uv_s = inr v_s⌝ ∗
-            l_t ↦{q_t}t v_t ∗ l_s ↦{q_s}s v_s }].
-  Proof.
-    iIntros (Hs Hτ_t Hτ_s) "Hl_t Hl_s".
-    iApply target_red_sim_expr.
-    iApply (target_red_load _ _ _ _ _ Hs Hτ_t with "Hl_t").
-    iIntros "Hl_t".
-
-    iApply source_red_sim_expr.
-    iApply (source_red_load _ _ _ _ _ Hs Hτ_s with "Hl_s").
-    iIntros "Hl_s".
-
-    iApply sim_expr_base. iExists _,_; iFrame.
-    repeat (iSplitL ""; [ done | ]).
-    rewrite !uvalue_to_dvalue_of_dvalue_to_uvalue; done.
-  Qed.
-
-  Lemma source_red_store1 v v' n i Ψ ptr:
-    ptr.1 ↦s [ LBlock n v i ] -∗
-    (ptr.1 ↦s [ LBlock n (add_all_index (serialize_dvalue v') ptr.2 v) i ] -∗
-      Ψ (Ret tt)) -∗
-    source_red (η := vir_handler) (trigger (Store (DVALUE_Addr ptr) v')) Ψ.
-  Proof.
-    rewrite source_red_unfold.
-    iIntros "Hs Hl". iLeft.
-    iIntros (σ_t σ_s) "SI".
-    iDestruct "SI" as (???) "(Hh_s & Hh_t & H_c & Hbij & SI)".
-
-    iDestruct (heap_read_st_1 with "Hh_s Hs") as %?; auto.
-    iPoseProof (heap_write with "Hh_s Hs") as ">(Hh_s & Hs)".
-    cbn. destruct ptr.
-    iSpecialize ("Hl" with "Hs").
-
-    iModIntro.
-    iExists _,tt,(fun x => Tau(Ret x)),_.
-    iSplitL ""; first iPureIntro.
-    { solve_eq.
-      apply get_logical_block_logical_view in H. rewrite /write.
-      rewrite /vir_heap in H. rewrite /get_logical_block /get_logical_block_mem.
-      rewrite H; cbn. by solve_eq. }
-
-    iSplitR "Hl"; last final; sfinal.
-
-    cbn; rewrite <- vir_heap_add_logical_block. cbn.
-    rewrite /dvalue_to_block.
-    cbn in *. rewrite /frames; cbn; eauto.
-    destruct_HC "Hh_s".
-
-    assert ({[ z ]} ∪ (vmem σ_s).1.2 = (vmem σ_s).1.2).
-    { destruct Hbs. cbn in *.
-      specialize (H1 z (ltac:(rewrite lookup_insert; eauto))).
-      destruct H1. set_solver. }
-
-    destruct (vmem σ_s); destruct f; cbn in *;
-    rewrite H0; sfinal.
-  Qed.
-
-  Lemma source_red_store v v' l Ψ:
-    length (serialize_dvalue v) = length (serialize_dvalue v') ->
-    l ↦s v -∗
-    (l ↦s v' -∗ Ψ (Ret tt)) -∗
-    source_red (η := vir_handler) (trigger (Store (# l) v')) Ψ.
-  Proof.
-    rewrite source_red_unfold.
-    iIntros (Hlen) "Hs Hl". iLeft.
-    iIntros (σ_t σ_s) "SI".
-    iDestruct "SI" as (???) "(Hh_s & Hh_t & H_c & Hbij & SI)".
-
-    iDestruct (heap_read with "Hh_s Hs") as %?; auto.
-    rewrite mapsto_dval_eq /mapsto_dval_def.
-    iPoseProof (heap_write with "Hh_s Hs") as ">(Hh_s & Hs)".
-    cbn; iSpecialize ("Hl" with "Hs").
-
-    iModIntro. iExists _,tt,(fun x => Tau (Ret x)),_.
-    iSplitL ""; first iPureIntro.
-    { solve_eq.
-      rewrite /write; rewrite get_logical_block_logical_view in H.
-      rewrite H. by solve_eq. }
-
-    iSplitR "Hl"; last final; sfinal.
-
-    cbn; rewrite <- vir_heap_add_logical_block.
-    rewrite /dvalue_to_block.
-    apply Nat2Z.inj_iff in Hlen. do 2 rewrite <- Zlength_correct in Hlen.
-
-    epose proof (@add_all_index_twice _ _ _ _ _ 0
-        (init_block (N.of_nat (length (serialize_dvalue v)))) Hlen).
-    apply leibniz_equiv in H0. rewrite H0.
-    rewrite !Zlength_correct in Hlen.
-    apply Nat2Z.inj in Hlen. rewrite Hlen.
-    rewrite /frames.
-    destruct (vmem σ_s) ; cbn in *.
-
-    destruct_HC "Hh_s".
-
-    assert ({[ l ]} ∪ p.2 = p.2).
-    { destruct Hbs. cbn in *.
-      destruct p. cbn in *.
-      specialize (H2 l (ltac:(rewrite lookup_insert; eauto))).
-      set_solver. }
-    rewrite H1.
-    sfinal.
-  Qed.
-
-  Lemma target_red_store1 v v' n i Ψ ptr:
+  Lemma target_store_block v v' n i Ψ ptr:
     ptr.1 ↦t [ LBlock n v i ] -∗
     (ptr.1 ↦t [ LBlock n (add_all_index (serialize_dvalue v') ptr.2 v) i ] -∗
       Ψ (Ret tt)) -∗
@@ -485,7 +551,7 @@ Section proof.
     rewrite H0. sfinal.
   Qed.
 
-  Lemma target_red_store v v' l Ψ:
+  Lemma target_store v v' l Ψ:
     length (serialize_dvalue v) = length (serialize_dvalue v') ->
     l ↦t v -∗
     (l ↦t v' -∗ Ψ (Ret tt)) -∗
@@ -531,49 +597,14 @@ Section proof.
     rewrite H1. sfinal.
   Qed.
 
-  Definition update_mem (b : logical_block) (f : mem_block -> mem_block) : logical_block :=
-    match b with
-      | LBlock n m i => LBlock n (f m) i
-    end.
-
-  Corollary source_red_store2 b v' Ψ ptr:
-    ptr.1 ↦s [ b ] -∗
-    (ptr.1 ↦s [ update_mem b
-                  (fun v => add_all_index (serialize_dvalue v') ptr.2 v) ] -∗
-      Ψ (Ret tt)) -∗
-    source_red (η := vir_handler) (trigger (Store (DVALUE_Addr ptr) v')) Ψ.
-  Proof.
-    destruct b.
-    iApply source_red_store1.
-  Qed.
-
-  Corollary target_red_store2 b v' Ψ ptr:
+  Corollary target_store_block1 b v' Ψ ptr:
     ptr.1 ↦t [ b ] -∗
-    (ptr.1 ↦t [ update_mem b
+    (ptr.1 ↦t [ update_block b
                   (fun v => add_all_index (serialize_dvalue v') ptr.2 v) ] -∗
       Ψ (Ret tt)) -∗
     target_red (η := vir_handler) (trigger (Store (DVALUE_Addr ptr) v')) Ψ.
   Proof.
-    destruct b.
-    iApply target_red_store1.
-  Qed.
-
-  Lemma sim_store v_t v_s v_t' v_s' l_t l_s:
-    length (serialize_dvalue v_t) = length (serialize_dvalue v_t') ->
-    length (serialize_dvalue v_s) = length (serialize_dvalue v_s') ->
-    l_t ↦t v_t -∗ l_s ↦s v_s -∗
-      trigger (Store (# l_t) v_t') ⪯ trigger (Store (# l_s) v_s')
-      [{ (v_t, v_s), l_t ↦t v_t' ∗ l_s ↦s v_s' }].
-  Proof.
-    iIntros (Hlen_t Hlen_s) "Hl_t Hl_s".
-    iApply target_red_sim_expr.
-    iApply (target_red_store _ _ _ _ Hlen_t with "Hl_t").
-    iIntros "Hl_t".
-
-    iApply source_red_sim_expr.
-    iApply (source_red_store _ _ _ _ Hlen_s with "Hl_s").
-    iIntros "Hl_s".
-    vfinal.
+    destruct b; iApply target_store_block.
   Qed.
 
   Lemma target_local_read (x : LLVMAst.raw_id) (v : uvalue) i Ψ:
@@ -608,37 +639,142 @@ Section proof.
     repeat iExists _; rewrite Hσ_t. by iFrame.
   Qed.
 
-  Lemma source_local_read (x : LLVMAst.raw_id) (v : uvalue) i Ψ:
-    ⊢ [x := v]s i -∗
-      stack_src i -∗
-      ([x := v]s i -∗
-        stack_src i -∗
-        Ψ (Ret v)) -∗
-      source_red (η := vir_handler) (trigger (LocalRead x)) Ψ.
+  (* TODO: Term [alloc] is misleading; rename *)
+  Lemma target_local_write_alloc
+    (x : LLVMAst.raw_id) (v : uvalue) L i Φ :
+    x ∉ L ->
+    ⊢ ldomain_tgt i L -∗
+      stack_tgt i -∗
+      ([ x := v ]t i -∗
+        ldomain_tgt i ({[x]} ∪ L) -∗
+          stack_tgt i -∗
+          Φ (Ret tt)) -∗
+      target_red (η := vir_handler) (trigger (LocalWrite x v)) Φ.
   Proof.
-    rewrite source_red_unfold.
-    iIntros "Hl Hf H".
-    iLeft.
+    rewrite target_red_unfold .
+    iIntros (Hlen) "Hd Hf Hl"; iLeft.
     iIntros (σ_t σ_s) "SI".
 
     iDestruct "SI" as (???) "(Hh_s & Hh_t & H_c & Hbij & SI)".
+    destruct (vlocal σ_t) eqn: Hlocal_t.
 
-    iDestruct (lheap_lookup with "Hh_s Hf Hl") as %Ht.
-    rewrite -alist_find_to_map_Some in Ht.
+    iExists _,
+      (update_local (alist_add x v l, l0) σ_t),
+      (fun x => Tau (Ret tt)),_.
 
-    iExists _, v, (fun x => Tau(Ret x)), _.
-
-    destruct (vlocal σ_s) eqn: Hσ_s.
     iSplitL ""; first iPureIntro.
-    { solve_eq.
-      rewrite Hσ_s. cbn. rewrite Ht.
-      solve_eq.
-      by rewrite -Hσ_s update_local_id. }
+    { solve_eq; rewrite Hlocal_t; by solve_eq. }
 
-    iSpecialize ("H" with "Hl Hf").
-    iSplitR "H"; last final.
+    iMod ((lheap_domain_alloc _ _ v)
+           with "Hd Hf Hh_t") as "(Hh_t & Hp_t & Hf_t & Hd_t)"; [done | ].
 
-    repeat iExists _; rewrite Hσ_s; by iFrame.
+    iDestruct (lheap_lookup with "Hh_t Hf_t Hp_t") as %Hl_t; cbn; iFrame.
+
+    iSpecialize ("Hl" with "Hp_t Hd_t Hf_t"); iFrame.
+    iSplitR "Hl"; last final; sfinal.
+  Qed.
+
+  Lemma target_local_write
+    (x : LLVMAst.raw_id) (v v' : uvalue) i Φ :
+    ⊢ [ x := v' ]t i -∗
+      stack_tgt i -∗
+      ([ x := v ]t i -∗
+          stack_tgt i -∗
+          Φ (Ret tt)) -∗
+      target_red (η := vir_handler) (trigger (LocalWrite x v)) Φ.
+  Proof.
+    rewrite target_red_unfold.
+    iIntros "Hx Hf Hl"; iLeft; iIntros (σ_t σ_s) "SI".
+
+    iDestruct "SI" as (???) "(Hh_s & Hh_t & H_c & Hbij & SI)".
+    destruct (vlocal σ_t) eqn: Hlocal_t.
+
+    iExists _,
+      (update_local (alist_add x v l, l0) σ_t),
+      (fun x => Tau (Ret tt)),_.
+
+    iSplitL ""; first iPureIntro.
+    { solve_eq. rewrite Hlocal_t. by solve_eq. }
+
+    iMod ((lheap_write _ _ _ v) with "Hh_t Hf Hx") as "(Hh_t & Hf & Hx)".
+
+    iDestruct (lheap_lookup with "Hh_t Hf Hx") as %Hl_t; cbn.
+
+    iSpecialize ("Hl" with "Hx Hf"); iFrame.
+    iSplitR "Hl"; last final; sfinal.
+  Qed.
+
+  (* ------------------------------------------------------------------------ *)
+  (* Simulation primitive laws on instruction-related events *)
+  (* ------------------------------------------------------------------------ *)
+
+  Lemma sim_alloca τ S_t S_s i_t i_s `{non_void τ}:
+    alloca_tgt i_t S_t -∗
+    alloca_src i_s S_s -∗
+    stack_tgt i_t -∗
+    stack_src i_s -∗
+    trigger (Alloca τ) ⪯ trigger (Alloca τ)
+      [{ (a, a0),
+          ∃ l_t l_s,
+            ⌜a = DVALUE_Addr (l_t, 0%Z)⌝ ∗ ⌜a0 = DVALUE_Addr (l_s, 0%Z)⌝ ∗
+            ⌜l_t ∉ S_t⌝ ∗ ⌜l_s ∉ S_s⌝ ∗
+            l_t ↦t [ make_empty_logical_block τ ] ∗
+            l_s ↦s [ make_empty_logical_block τ ] ∗
+            alloca_tgt i_t ({[l_t]} ∪ S_t) ∗
+            alloca_src i_s ({[l_s]} ∪ S_s) ∗
+            stack_tgt i_t ∗
+            stack_src i_s ∗
+            target_block_size l_t (Some (N.to_nat (sizeof_dtyp τ))) ∗
+            source_block_size l_s (Some (N.to_nat (sizeof_dtyp τ)))}].
+  Proof.
+    iIntros "Hl_t Hl_s Hf_t Hf_s".
+    iApply target_red_sim_expr.
+    iApply (target_alloca with "Hl_t Hf_t"); [ done | ].
+    iIntros (??) "Hl_t Ha_t Hf_t Hb_t".
+
+    iApply source_red_sim_expr.
+    iApply (source_alloca with "Hl_s Hf_s"); [ done | ].
+    iIntros (??) "Hl_s Ha_s Hf_s Hb_s".
+    vfinal; sfinal.
+  Qed.
+
+  Lemma sim_load l_t l_s τ v_t v_s q_t q_s:
+    is_supported τ ->
+    dvalue_has_dtyp v_t τ  ->
+    dvalue_has_dtyp v_s τ  ->
+    l_t ↦{q_t}t v_t -∗ l_s ↦{q_s}s v_s -∗
+    trigger (Load τ (# l_t)) ⪯ trigger (Load τ (# l_s))
+      [{ (uv_t, uv_s),
+            ⌜uvalue_to_dvalue uv_t = inr v_t⌝ ∗
+            ⌜uvalue_to_dvalue uv_s = inr v_s⌝ ∗
+            l_t ↦{q_t}t v_t ∗ l_s ↦{q_s}s v_s }].
+  Proof.
+    iIntros (Hs Hτ_t Hτ_s) "Hl_t Hl_s".
+    iApply target_red_sim_expr.
+    iApply (target_load _ _ _ _ _ Hs Hτ_t with "Hl_t").
+    iIntros "Hl_t".
+
+    iApply source_red_sim_expr.
+    iApply (source_load _ _ _ _ _ Hs Hτ_s with "Hl_s").
+    iIntros "Hl_s"; vfinal.
+    by rewrite !uvalue_to_dvalue_of_dvalue_to_uvalue.
+  Qed.
+
+  Lemma sim_store v_t v_s v_t' v_s' l_t l_s:
+    length (serialize_dvalue v_t) = length (serialize_dvalue v_t') ->
+    length (serialize_dvalue v_s) = length (serialize_dvalue v_s') ->
+    l_t ↦t v_t -∗ l_s ↦s v_s -∗
+      trigger (Store (# l_t) v_t') ⪯ trigger (Store (# l_s) v_s')
+      [{ (v_t, v_s), l_t ↦t v_t' ∗ l_s ↦s v_s' }].
+  Proof.
+    iIntros (Hlen_t Hlen_s) "Hl_t Hl_s".
+    iApply target_red_sim_expr.
+    iApply (target_store _ _ _ _ Hlen_t with "Hl_t").
+    iIntros "Hl_t".
+
+    iApply source_red_sim_expr.
+    iApply (source_store _ _ _ _ Hlen_s with "Hl_s").
+    iIntros "Hl_s"; vfinal.
   Qed.
 
   Lemma sim_local_read (x_t x_s : LLVMAst.raw_id) (v_t v_s : uvalue) i_t i_s:
@@ -658,9 +794,7 @@ Section proof.
 
     iApply source_red_sim_expr.
     iApply (source_local_read with "Hs Hf_s").
-    iIntros "Hs Hf_s".
-
-    vfinal.
+    iIntros "Hs Hf_s"; vfinal.
   Qed.
 
   Lemma sim_local_read_not_in_domain {R} (x_s : LLVMAst.raw_id) L_s Φ (e_t : _ R) i:
@@ -697,108 +831,6 @@ Section proof.
     intros; inversion H.
   Qed.
 
-  (* TODO: Term [alloc] is misleading; rename *)
-  Lemma target_local_write_alloc
-    (x : LLVMAst.raw_id) (v : uvalue) L i Φ :
-    x ∉ L ->
-    ⊢ ldomain_tgt i L -∗
-      stack_tgt i -∗
-      ([ x := v ]t i -∗
-        ldomain_tgt i ({[x]} ∪ L) -∗
-          stack_tgt i -∗
-          target_red (η := vir_handler) (Ret tt) Φ) -∗
-      target_red (η := vir_handler) (trigger (LocalWrite x v)) Φ.
-  Proof.
-    setoid_rewrite target_red_unfold at 2.
-    iIntros (Hlen) "Hd Hf Hl".
-    iLeft.
-    iIntros (σ_t σ_s) "SI".
-
-    iDestruct "SI" as (???) "(Hh_s & Hh_t & H_c & Hbij & SI)".
-    destruct (vlocal σ_t) eqn: Hlocal_t.
-
-    iExists _,
-      (update_local (alist_add x v l, l0) σ_t),
-      (fun x => Tau (Ret tt)),_.
-
-    iSplitL "".
-    { unfold interp_L2. rewrite interp_state_vis.
-      cbn.
-      rewrite
-        /resum /ReSum_inr /cat /Cat_IFun /inr_ /Inr_sum1 /add_tau /case_; cbn.
-      rewrite Hlocal_t.
-      rewrite bind_bind. rewrite !bind_ret_l.
-      iPureIntro.
-      setoid_rewrite interp_state_ret. rewrite !bind_tau.
-      rewrite !bind_ret_l.
-      apply eqit_Tau. cbn.
-      rewrite interp_state_tau interp_state_ret.
-      reflexivity. }
-
-    (* Ned to go back to repair *)
-    iMod ((lheap_domain_alloc _ _ v)
-           with "Hd Hf Hh_t") as "(Hh_t & Hp_t & Hf_t & Hd_t)"; [done | ].
-
-    iDestruct (lheap_lookup with "Hh_t Hf_t Hp_t") as %Hl_t.
-    cbn. iFrame.
-
-    iSpecialize ("Hl" with "Hp_t Hd_t Hf_t"); iFrame.
-    iSplitR "Hl"; cycle 1.
-    { by iApply target_red_tau. }
-
-    repeat iExists _; by iFrame.
-  Qed.
-
-  Lemma source_local_write_alloc
-    (x : LLVMAst.raw_id) (v : uvalue) L i Φ :
-    x ∉ L ->
-    ⊢ ldomain_src i L -∗
-      stack_src i -∗
-      ([ x := v ]s i -∗
-        ldomain_src i ({[x]} ∪ L) -∗
-          stack_src i -∗
-          source_red (η := vir_handler) (Ret tt) Φ) -∗
-      source_red (η := vir_handler) (trigger (LocalWrite x v)) Φ.
-  Proof.
-    setoid_rewrite source_red_unfold at 2.
-    iIntros (Hlen) "Hd Hf Hl".
-    iLeft.
-    iIntros (σ_t σ_s) "SI".
-
-    iDestruct "SI" as (???) "(Hh_s & Hh_t & H_c & Hbij & SI)".
-    destruct (vlocal σ_s) eqn: Hlocal_s.
-
-    iExists _,
-      (update_local (alist_add x v l, l0) σ_s),
-      (fun x => Tau (Ret tt)),_.
-
-    iSplitL "".
-    { unfold interp_L2. rewrite interp_state_vis.
-      cbn.
-      rewrite
-        /resum /ReSum_inr /cat /Cat_IFun /inr_ /Inr_sum1 /add_tau /case_; cbn.
-      rewrite Hlocal_s.
-      rewrite bind_bind. rewrite !bind_ret_l.
-      iPureIntro.
-      setoid_rewrite interp_state_ret. rewrite !bind_tau.
-      rewrite !bind_ret_l.
-      apply eqit_Tau. cbn.
-      rewrite interp_state_tau interp_state_ret.
-      reflexivity. }
-
-    iMod ((lheap_domain_alloc _ _ v)
-           with "Hd Hf Hh_s") as "(Hh_s & Hp_s & Hf_s & Hd_s)"; [done | ].
-
-    iDestruct (lheap_lookup with "Hh_s Hf_s Hp_s") as %Hl_s.
-    cbn. iFrame.
-
-    iSpecialize ("Hl" with "Hp_s Hd_s Hf_s"); iFrame.
-    iSplitR "Hl"; cycle 1.
-    { by iApply source_red_tau. }
-
-    repeat iExists _; by iFrame.
-  Qed.
-
   Lemma sim_local_write_alloc
     (x_t x_s : LLVMAst.raw_id) (v_t v_s : uvalue) L_t L_s i_t i_s:
     x_t ∉ L_t ->
@@ -811,132 +843,16 @@ Section proof.
           ldomain_tgt i_t ({[x_t]} ∪ L_t) ∗ ldomain_src i_s ({[x_s]} ∪ L_s)
           ∗ stack_tgt i_t ∗ stack_src i_s }].
   Proof.
-    rewrite sim_expr_unfold.
+    iIntros (Ht Hs) "Hl_t Hl_s Hs_t Hs_s".
+    iApply target_red_sim_expr.
+    iApply (target_local_write_alloc _ _ _ _ _ Ht with "Hl_t Hs_t").
+    iIntros "Ht Hl_t Hs_t".
 
-    iIntros (Ht Hs) "Ht Hs Hf_t Hf_s %σ_t %σ_s SI".
-    cbn. destruct (vlocal σ_t), (vlocal σ_s).
-
-    rewrite /interp_L2;
-    provide_case: TAU_STEP.
-
-    rewrite sim_coindF_unfold sim_indF_unfold /sim_expr_inner.
-
-    provide_case: TAU_STEP. cbn.
-    do 2 (iSplitL ""; [ done | ]).
-
-    iDestruct "SI" as (???) "(Hh_s&Hh_t&HC&Hbij&Hg)".
-    cbn.
-    rewrite sim_coindF_unfold sim_indF_unfold /sim_expr_inner.
-
-    iMod ((lheap_domain_alloc _ _ v_t) with "Ht Hf_t Hh_t") as "(Hh_t & Hp_t & Hf_t & Hd_t)"; [done | ].
-    iMod ((lheap_domain_alloc _ _ v_s) with "Hs Hf_s Hh_s") as "(Hh_s & Hp_s & Hf_s & Hd_s)"; [done | ].
-
-    iDestruct (lheap_lookup with "Hh_t Hf_t Hp_t") as %Hl_t.
-    iDestruct (lheap_lookup with "Hh_s Hf_s Hp_s") as %Hl_s.
-    cbn.
-    provide_case: BASE; iFrame.
-    iSplitR ""; [ cbn; rewrite /state_interp; repeat iExists _; iFrame | ].
-
-    repeat iExists _; by iFrame.
+    iApply source_red_sim_expr.
+    iApply (source_local_write_alloc _ _ _ _ _ Hs with "Hl_s Hs_s").
+    iIntros "Hs Hl_s Hs_s";
+    vfinal.
   Qed.
-
-  Lemma target_local_write
-    (x : LLVMAst.raw_id) (v v' : uvalue) L i Φ :
-    ⊢ [ x := v' ]t i -∗
-      ldomain_tgt i L -∗
-      stack_tgt i -∗
-      ([ x := v ]t i -∗
-        ldomain_tgt i L -∗
-          stack_tgt i -∗
-          target_red (η := vir_handler) (Ret tt) Φ) -∗
-      target_red (η := vir_handler) (trigger (LocalWrite x v)) Φ.
-  Proof.
-    setoid_rewrite target_red_unfold at 2.
-    iIntros "Hx Hd Hf Hl".
-    iLeft; iIntros (σ_t σ_s) "SI".
-
-    iDestruct "SI" as (???) "(Hh_s & Hh_t & H_c & Hbij & SI)".
-    destruct (vlocal σ_t) eqn: Hlocal_t.
-
-    iExists _,
-      (update_local (alist_add x v l, l0) σ_t),
-      (fun x => Tau (Ret tt)),_.
-
-    iSplitL "".
-    { unfold interp_L2. rewrite interp_state_vis.
-      cbn.
-      rewrite
-        /resum /ReSum_inr /cat /Cat_IFun /inr_ /Inr_sum1 /add_tau /case_; cbn.
-      rewrite Hlocal_t.
-      rewrite bind_bind. rewrite !bind_ret_l.
-      iPureIntro.
-      setoid_rewrite interp_state_ret. rewrite !bind_tau.
-      rewrite !bind_ret_l.
-      apply eqit_Tau. cbn.
-      rewrite interp_state_tau interp_state_ret.
-      reflexivity. }
-
-    iMod ((lheap_write _ _ _ v) with "Hh_t Hf Hx") as "(Hh_t & Hf & Hx)".
-
-    iDestruct (lheap_lookup with "Hh_t Hf Hx") as %Hl_t.
-    cbn.
-
-    iSpecialize ("Hl" with "Hx Hd Hf"); iFrame.
-    iSplitR "Hl"; cycle 1.
-    { by iApply target_red_tau. }
-
-    repeat iExists _; by iFrame.
-  Qed.
-
-  Lemma source_local_write
-    (x : LLVMAst.raw_id) (v v' : uvalue) L i Φ :
-    ⊢ [ x := v' ]s i -∗
-      ldomain_src i L -∗
-      stack_src i -∗
-      ([ x := v ]s i -∗
-        ldomain_src i L -∗
-          stack_src i -∗
-          source_red (η := vir_handler) (Ret tt) Φ) -∗
-      source_red (η := vir_handler) (trigger (LocalWrite x v)) Φ.
-  Proof.
-    setoid_rewrite source_red_unfold at 2.
-    iIntros "Hx Hd Hf Hl".
-    iLeft.
-    iIntros (σ_t σ_s) "SI".
-
-    iDestruct "SI" as (???) "(Hh_s & Hh_t & H_c & Hbij & SI)".
-    destruct (vlocal σ_s) eqn: Hlocal_s.
-
-    iExists _,
-      (update_local (alist_add x v l, l0) σ_s),
-      (fun x => Tau (Ret tt)),_.
-
-    iSplitL "".
-    { unfold interp_L2. rewrite interp_state_vis.
-      cbn.
-      rewrite
-        /resum /ReSum_inr /cat /Cat_IFun /inr_ /Inr_sum1 /add_tau /case_; cbn.
-      rewrite Hlocal_s.
-      rewrite bind_bind. rewrite !bind_ret_l.
-      iPureIntro.
-      setoid_rewrite interp_state_ret. rewrite !bind_tau.
-      rewrite !bind_ret_l.
-      apply eqit_Tau. cbn.
-      rewrite interp_state_tau interp_state_ret.
-      reflexivity. }
-
-    iMod ((lheap_write _ _ _ v) with "Hh_s Hf Hx") as "(Hh_s & Hf & Hx)".
-
-    iDestruct (lheap_lookup with "Hh_s Hf Hx") as %Hl_s.
-    cbn.
-
-    iSpecialize ("Hl" with "Hx Hd Hf"); iFrame.
-    iSplitR "Hl"; cycle 1.
-    { by iApply source_red_tau. }
-
-    repeat iExists _; by iFrame.
-  Qed.
-
 
   (* Ghost resource doesn't check that it gets assigned only once. It must be a
     well-formed LLVM IR program. *)
@@ -948,33 +864,14 @@ Section proof.
           [ x_t := v_t' ]t i_t ∗ [ x_s := v_s' ]s i_s ∗
           stack_tgt i_t ∗ stack_src i_s}].
   Proof.
-    rewrite sim_expr_unfold.
+    iIntros  "Hs_t Hs_s Ht Hs".
+    iApply target_red_sim_expr.
+    iApply (target_local_write with "Ht Hs_t").
+    iIntros "Ht Hs_t".
 
-    iIntros "Hf_t Hf_s Ht Hs %σ_t %σ_s SI".
-    rewrite /interp_L2;
-    provide_case: TAU_STEP.
-    (iSplitL ""; [ iPureIntro | ]).
-    { apply Eq.EqAxiom.bisimulation_is_eq. cbn; reflexivity. }
-    (iSplitL ""; [ iPureIntro | ]).
-    { apply Eq.EqAxiom.bisimulation_is_eq. cbn; reflexivity. }
-
-    destruct (vlocal σ_t) eqn: Hlocal_t; destruct (vlocal σ_s) eqn: Hlocal_s.
-    rewrite sim_coindF_unfold sim_indF_unfold /sim_expr_inner.
-
-    cbn.
-    provide_case: TAU_STEP. cbn.
-    iDestruct "SI" as (???) "(Hh_s&Hh_t&HC&Hbij&Hg)".
-    rewrite sim_coindF_unfold sim_indF_unfold /sim_expr_inner.
-
-    iMod (lheap_write with "Hh_t Hf_t Ht") as "(Hh_t & Hf_t & Ht)".
-    iMod (lheap_write with "Hh_s Hf_s Hs") as "(Hh_s & Hf_s & Hs)".
-    provide_case:BASE.
-
-    rewrite /lift_expr_rel; cbn; iFrame.
-    iSplitR ""; cycle 1.
-    { repeat iExists _; done. }
-    iExists C, S, G; iFrame. rewrite Hlocal_t Hlocal_s; iFrame.
+    iApply source_red_sim_expr.
+    iApply (source_local_write with "Hs Hs_s").
+    iIntros "Hs Hs_s"; vfinal.
   Qed.
 
-End proof.
-
+End primitive_rules.
